@base  <http://www.daisy.org/z3986/2010/vocab/core/> .
@prefix rdf:  <http://www.w3.org/1999/02/22-rdf-syntax-ns#> .
@prefix rdfs: <http://www.w3.org/2000/01/rdf-schema#> .
@prefix owl:  <http://www.w3.org/2002/07/owl#> .
@prefix dcterms:  <http://purl.org/dc/terms/> .
@prefix : <#> .

<> 
  dcterms:title "Z39-86 2010 Core Vocabulary - Structural Semantics of Written Works";
  dcterms:publisher "DAISY Consortium";
  dcterms:creator "mgylling";
  dcterms:creator "mdemeglio";
  dcterms:date "2009-12-01" .

########################################
########## major sectioning ############
########################################

:Section a rdf:class ;
		owl:disjointWith :Block .

:frontmatter a rdf:Property ; 
		rdfs:label "frontmatter" ;
		rdfs:subPropertyOf :section ;
		rdfs:comment "TODO" .

:bodymatter a rdf:Property ; 
		rdfs:label "frontmatter" ;
		rdfs:subPropertyOf :section ;
		rdfs:comment "TODO" .
		
:backmatter a rdf:Property ; 
		rdfs:label "backmatter" ;
		rdfs:subPropertyOf :section ;
		rdfs:comment "TODO" .

:section a rdf:Property;
  		rdfs:label "section" ;
  		rdfs:domain :Section ;
  		rdfs:comment "A generic structural division of content" .
  
:part a rdf:Property;  
		rdfs:label "part" ;
		rdfs:subPropertyOf :section ; 		 
		rdfs:comment "A major structural division of a piece of writing, typically encapsulating a set of related chapters" .

:chapter a rdf:Property ; 
		rdfs:label "chapter" ;	
		rdfs:subPropertyOf :section ;
		rdfs:comment "A major structural division of a piece of writing" .

:article a rdf:Property ; 
		rdfs:label "article" ;
		rdfs:subPropertyOf :section ;
		rdfs:comment "A major independent section in a piece of writing, typically appearing in journals, magazines or newspapers" .

:foreword a rdf:Property ;
		rdfs:label "foreword" ;
		rdfs:subPropertyOf :section ;
		rdfs:comment "An introductory section in the beginning of the work, typically written by someone else than the work's author" .

:preface a rdf:Property ;
		rdfs:label "preface" ;
		rdfs:subPropertyOf :section ;
		rdfs:comment "An introductory section in the beginning of the work, typically written by the work's author" .
	
:introduction a rdf:Property ;
		rdfs:label "introduction" ;
		rdfs:subPropertyOf :section ;
		rdfs:comment "A section in the beginning of the work, typically introducing the reader to the scope or nature of the work's content". 

:preamble a rdf:Property ;
		rdfs:label "preamble" ;
		rdfs:subPropertyOf :introduction ;
		rdfs:comment "A section in the beginning of the work, typically containing introductory and/or explanatory prose regarding the scope or nature of the work's content".

:toc a rdf:Property ;
		rdfs:label "toc" ;
		rdfs:subPropertyOf :section ;
		rdfs:comment "A table of contents, typically appearing in the work's frontmatter, or at the beginning of a section" .
	
:epilogue a rdf:Property ;
		rdfs:label "epilogue" ;
		rdfs:subPropertyOf :section ;
		rdfs:comment "An ending section, part of the narrative" . 

:afterword a rdf:Property ;
		rdfs:label "afterword" ;
		rdfs:subPropertyOf :section ;
		rdfs:comment "An ending section, not part of the narrative" .
	
:conclusion a rdf:Property ;
		rdfs:label "conclusion" ;
		rdfs:subPropertyOf :section ;
		rdfs:comment "An ending section, typically containing statements concluding the work" .


########################################
############ block sectioning ##########
########################################

:Block a rdf:class ;
		owl:disjointWith :Section .
				
:block a rdf:Property ;
  		rdfs:label "block" ;
  		rdfs:domain :Block ;
  		rdfs:comment "A generic block of content, always subordinate to a Section" ;
  		dcterms:description "A block does not necessarily represent anything nameable in itself, and will in these cases merely create an association between its descendants" .
  		
:para a rdf:Property ;  
		rdfs:label "para" ;
		rdfs:subPropertyOf :block ; 		 
		rdfs:comment "A paragraph, consisting of one or several sentences, preceded by an empty line in the main body of text, with the first line of the paragraph sometimes indented" .  		
  		
:linegroup a rdf:Property ;  
		rdfs:label "linegroup" ;
		rdfs:subPropertyOf :block ; 		 
		rdfs:comment "A group of lines" .

:note a rdf:Property ;  
		rdfs:label "note" ;
		rdfs:subPropertyOf :block ; 		 
		rdfs:comment "A footnote or a rearnote, typically linked from the main text via a note reference" .

:footnotes a rdf:Property ;  
		rdfs:label "footnotes" ;
		rdfs:subPropertyOf :block ; # TODO and Collection		
		rdfs:seeAlso :footnote; 
		rdfs:comment "A collection of notes appearing at the bottom of a page" .

:footnote a rdf:Property ;  
		rdfs:label "footnote" ;
		rdfs:subPropertyOf :note ; 		 
		rdfs:seeAlso :footnotes;
		rdfs:comment "A note appearing at the bottom of a page" .
		
:rearnote a rdf:Property ;  
		rdfs:label "rearnote" ;
		rdfs:subPropertyOf :note ; 	
		rdfs:seeAlso :rearnotes;	 
		rdfs:comment "A note appearing in the rear (backmatter) of the work, or at the end of a section" .

############ asides ##########

:Aside a rdf:class ;
		rdfs:subclassOf :Block .
		
:aside a rdf:Property ;
		rdfs:label "aside" ;
		rdfs:domain :Aside ;
		rdfs:comment "Secondary or supplementary content" .

:sidebar a rdf:Property ;
		rdfs:label "sidebar" ;
		rdfs:subPropertyOf :aside ;
		rdfs:comment "Secondary or supplementary content, typically formatted as an inset or box" .

:practice a rdf:Property ;
		rdfs:label "practice" ;
		rdfs:subPropertyOf :aside ;
		rdfs:comment "A review exercise or sample" .

:notice a rdf:Property ;
		rdfs:label "notice" ;
		rdfs:subPropertyOf :aside ;
		rdfs:comment "A notification" .

:warning a rdf:Property ;
		rdfs:label "warning" ;
		rdfs:subPropertyOf :aside ;
		rdfs:comment "A warning" .

:marginalia a rdf:Property ;
		rdfs:label "marginalia" ;
		rdfs:subPropertyOf :aside ; #TODO and span
		rdfs:comment "Marginalia" .

########################################
###### backmatter sections/blocks ######
########################################

:appendix a rdf:Property ;
		rdfs:label "appendix";		
		rdfs:subPropertyOf :section ;
		rdfs:comment "Supplemental information" .

:glossary a rdf:Property ;
		rdfs:label "glossary";		
		rdfs:subPropertyOf :section ; # TODO and Collection
		rdfs:comment "An alphabetical list of terms in a particular domain of knowledge with the definitions for those terms" .
	 
:bibliography a rdf:Property ;
		rdfs:label "bibliography";		
		rdfs:subPropertyOf :section ; # TODO and Collection
		rdfs:comment "A systematic list of cited works" .

:index a rdf:Property ;
		rdfs:label "index";		
		rdfs:subPropertyOf :section ; # TODO and Collection
		rdfs:comment "A detailed list, usually arranged alphabetically, of the specific information in a publication" .

:colophon a rdf:Property ;
		rdfs:label "colophon";		
		rdfs:subPropertyOf :section ;
		rdfs:comment "A brief description usually located at the end of a publication, describing production notes relevant to the edition" .
		
:rearnotes a rdf:Property ;
    	rdfs:label "rearnotes" ;		
		rdfs:seeAlso :rearnote ;
		rdfs:subPropertyOf :section ; # TODO and Collection
		rdfs:comment "A collection of notes appearing at the rear (backmatter) of the work, or at the end of a section" .


########################################
###### frontmatter sections/blocks #####
########################################

:titlepage
    	rdfs:label "titlepage" ;
		rdfs:subPropertyOf :section ; # TODO and block
		rdfs:comment "The title page of the work" .

:halftitlepage
    	rdfs:label "halftitlepage" ;
    	rdfs:subPropertyOf :section ; # TODO and block
		rdfs:comment "The half-title page of the work" .

:dedication
    	rdfs:label "dedication" ;
		rdfs:subPropertyOf :section ; # TODO and block    	
		rdfs:comment "An inscription addressed to one or several particular person(s)" .

:epigraph
    	rdfs:label "epigraph" ;
		rdfs:subPropertyOf :section ; # TODO and block    	
		rdfs:comment "A quotation that is pertinent but not integral to the text" .

:acknowledgments
    	rdfs:label "acknowledgments" ;
		rdfs:subPropertyOf :section ; # TODO and block    	
		rdfs:comment "A passage containing acknowledgments to entities involved in the realization of the work" .

:imprint
    	rdfs:label "imprint" ;
		rdfs:subPropertyOf :block ;     	
		rdfs:comment "Information relating to the publication or distribution of the work" .

:imprimatur
    	rdfs:label "imprimatur" ;
		rdfs:subPropertyOf :block ;     	
		rdfs:comment "A formal statement authorizing the publication of the work" .
	
:publisher-address
    	rdfs:label "publisher-address" ;
    	rdfs:subPropertyOf :block ;
		rdfs:comment "The publisher's address, which can be abbreviated to city and postal code only" .

:grant-acknowledgment
    	rdfs:label "grant-acknowledgment" ;
    	rdfs:subPropertyOf :block ;    	
		rdfs:comment "Describes financial assistance towards the work" .

:contributors
    	rdfs:label "contributors" ;
    	rdfs:subPropertyOf :block, :list ;     	  	
		rdfs:comment "A list of contributors to the work" .
		
:other-credits
    	rdfs:label "other-credits" ;
    	rdfs:subPropertyOf :block ;    	
		rdfs:comment "Acknowledgments of previously published parts of the work, illustration credits, and permission to quote from copyrighted material" .
		 		
:biographical-note
    	rdfs:label "biographical-note" ;
    	rdfs:subPropertyOf :block ;    	
		rdfs:comment "A biographical note about the author or authors (“author” here includes editors, compilers, and translators)" .

:translator-note
		rdfs:label "translator-note" ;
    	rdfs:subPropertyOf :block ;		
		rdfs:comment "A note from the translator" .


########################################
################ verse #################
########################################	

:Verse a rdf:class ;
	rdfs:subclassOf :Section, :Block .	
	
#poem
#	A poem
#song


		
########################################
############### titles #################
########################################	

:Title a rdf:class .
	
:title a rdf:Property ;
		rdfs:label "title" ;
		rdfs:domain :Title ;
		owl:sameAs dcterms:title;
		rdfs:comment "The title of the work, or, when used in the context of a fulltitle, the primary part of the full title" .

:halftitle a rdf:Property ;
		rdfs:label "halftitle" ;
		rdfs:subPropertyOf :title ;
		rdfs:comment "The halftitle of the work" .

:fulltitle a rdf:Property ;
		rdfs:label "fulltitle" ;
		rdfs:subPropertyOf :title ;
		rdfs:comment "The fulltitle of the work" .

:subtitle a rdf:Property;
		rdfs:label "subtitle" ;
		rdfs:subPropertyOf :title ;
		rdfs:comment "The secondary part of the fulltitle of the work" .	


########################################
############### headings ###############
########################################	
	
:Heading a rdf:class .	
	
:heading a rdf:Property;
		rdfs:label "heading" ;
		rdfs:domain :Heading ;
		rdfs:comment "The title of a Section (part, chapter, subchapter, article, etc)" .	
	
:bridgehead a rdf:Property;
		rdfs:label "bridgehead" ;
		rdfs:subPropertyOf :heading ;
		rdfs:comment "A free-floating heading that is not associated with the hierarchical structure of a document" .


########################################
################ lists #################
########################################	
	
:Collection a rdf:class ;
		rdfs:subclassOf :Block .
	
:List a rdf:class ;
		rdfs:subclassOf :Collection .

:list a rdf:Property ;
		rdfs:label "list" ;
		rdfs:domain :List ;
		rdfs:comment "An ordered or unordered set of interrelated items" .	

:orderedlist a rdf:Property ;
		rdfs:label "orderedlist" ;
		rdfs:subPropertyOf :list ;	
		rdfs:comment "A list where the order of the list's items is significant" .
	
:unorderedlist a rdf:Property ;
		rdfs:label "unorderedlist" ;
		rdfs:subPropertyOf :list ;	
		rdfs:comment "A list where the order of the list's items is insignificant" .	
	
:abbreviations a rdf:Property ;
		rdfs:label "abbreviations" ;
		rdfs:subPropertyOf :unorderedlist ;
		rdfs:comment "A list of abbreviations" .

:definitions a rdf:Property ;
		rdfs:label "definitions" ;
		rdfs:subPropertyOf :unorderedlist ;
		rdfs:comment "A list of definitions (of terms, concepts)". 

:timeline a rdf:Property ;
		rdfs:label "timeline" ;
		rdfs:subPropertyOf :orderedlist ;
		rdfs:comment "A chronological list of events".
	

########################################
############## pagination ##############
########################################		
	
:pagebreak a rdf:Property ;
		rdfs:label "pagebreak" ;
		rdfs:comment "A separator denoting the position where a break between two contiguous pages occurs in a paginated media" .
		
:page-header a rdf:Property ;		
		rdfs:label "page-header" ;
		rdfs:subPropertyOf :block ;
		rdfs:comment "Material, separate from the main body of text, appearing at the top of a printed page" .
				
:page-footer a rdf:Property ;
		rdfs:label "page-footer" ;
		rdfs:subPropertyOf :block ;
		rdfs:comment "Material, separate from the main body of text, appearing at the bottom of a printed page" .
	
	
########################################
############# annotations ##############
########################################	

:Annotation a rdf:class ;
		rdfs:subclassOf :Block, :Aside .
	
:annotation a rdf:Property ;
		rdfs:label "annotation" ;
		rdfs:domain :Annotation ;
		rdfs:comment "Overlay information about passages in the work" .

:author-anno a rdf:Property ;
		rdfs:label "author-anno" ;
		rdfs:subPropertyOf :annotation ;
		rdfs:comment "An annotation contributed by an author of the work" .

:editor-anno a rdf:Property ;
		rdfs:label "editor-anno" ;
		rdfs:subPropertyOf :annotation ;
		rdfs:comment "An annotation contributed by an editor of the work" .

:commentator-anno a rdf:Property ;
		rdfs:label "commentator-anno" ;
		rdfs:subPropertyOf :annotation ;
		rdfs:comment "An annotation contributed by a commentator of the work" .

:translator-anno a rdf:Property ;
		rdfs:label "translator-anno" ;
		rdfs:subPropertyOf :annotation ;
		rdfs:comment "An annotation contributed by a translator of the work" .

:republisher-anno a rdf:Property ;
		rdfs:label "republisher-anno" ;
		rdfs:subPropertyOf :annotation, :custom ;
		rdfs:comment "An annotation contributed by a republisher" .
	
	
	
########################################
############# references ###############
########################################	

:Reference a rdf:class .

:reference a rdf:Property ;
		rdfs:label "reference" ;
		rdfs:domain :Reference ;
		rdfs:comment "A reference to another entity - a resource, fragment, concept, or notion" .

:resolving-reference a rdf:Property ;
		rdfs:label "resolving-reference" ;
		rdfs:subPropertyOf :reference ;
		rdfs:comment "A reference which contains data intended to allow resolving the target entity" .

:loose-reference a rdf:Property ;
		rdfs:label "loose-reference" ;
		rdfs:subPropertyOf :reference ;
		rdfs:comment "A reference to a non-resolving target - a concept, notion or other imprecisely defined entity" .

:noteref a rdf:Property ;
		rdfs:label "noteref" ;
		rdfs:subPropertyOf :resolving-reference ;
		rdfs:comment "A reference to a note, typically appearing a superscripted symbol in the main body of text" ;
		rdfs:seeAlso :note .

:annoref a rdf:Property ;
		rdfs:label "annoref" ;
		rdfs:subPropertyOf :resolving-reference ;
		rdfs:comment "A reference to an annotation" ;
		rdfs:seeAlso :annotation .
		
:citation a rdf:Property ;
		rdfs:label "citation" ;
		rdfs:subPropertyOf :resolving-reference ;
		rdfs:comment "A reference to bibliographic work, typically resolving to an entry in an identified bibliography" ;
		rdfs:seeAlso :loose-citation ;
		rdfs:seeAlso :bibliography .

:loose-citation a rdf:Property ;
		rdfs:label "loose-citation" ;		
		rdfs:subPropertyOf :loose-reference ;
		rdfs:seeAlso :citation ;
		rdfs:comment "An imprecise reference to a bibliographic work" .

:image-placeholder a rdf:Property ;
		rdfs:label "image-placeholder" ;
		rdfs:subPropertyOf :reference, :custom ;
		rdfs:comment "A placeholder for a reference to a non-existing or removed image" .


########################################
################# text #################
########################################	

:Text a rdf:class .

:span a rdf:Property ;
		rdfs:label "span" ;		
		rdfs:domain :Text ;
		rdfs:comment "A range of text" .	


########################################
################ lines #################
########################################	

:line a rdf:Property ;
		rdfs:label "line" .

:byline a rdf:Property ;
		rdfs:label "byline" .
		
:dateline a rdf:Property ;
		rdfs:label "dateline" .
		
		
########################################
########### custom content #############
########################################	

:Custom a rdf:class .

:custom a rdf:Property ;
	rdfs:domain :Custom ;
	rdfs:comment "Structures added or removed during republishing, thus representing a deviation from the source" ;
	dcterms:description "Typically used to adapt the content for a particular output format" .


################################################################################	
#pgroup
#tables
#illustration, artwork
#for verse: poem, song/lyrics, hymn -- load of poetry measures for verse, in dedicated vocab
#byline, dateline
#georges sentence stuff on wiki
#word-->keyword
#dramatis personœ, persona
#
#decorative (to set on say an image to indicate that it does not contain content, just layout/typographic/stylisting/rendition) role="rend"	
#errata
#	errata
#essay, book etc
#
#diary
#	A diary
#
#diaryEntry
#	A diary entry
#
#issue 52: letter properties
#letter
#	A letter
#
#
#promotional-copy
#	A description of the book or quotations from reviews
#
#help
#	Help using the publication.
#
#keyword
#	A key word or phrase
#
#	
#body-artwork
#	Bodymatter artwork
# A headline is text at the top of a newspaper article, indicating the nature of the article below it.
# what/where? from frontmatter
#:publisher-logo
#    	rdfs:label "publisher-logo" ;
#		rdfs:subPropertyOf :??? ;     	
#		rdfs:comment "The publisher's logo" .
#		#TODO reference?
#:cover-artwork
#    	rdfs:label "cover-artwork" ;
#		rdfs:comment "Cover artwork" .
